theories/lithium/simpl_classes.v
@@ -10,12 +10,13 @@ Class SimplForall (T : Type) (n : nat) (e : T → Prop) (Q: Prop) := simpl_foral
 (** * [SimplImpl] and [SimplAnd] *)
 
 (** ** [SimplImplUnsafe] and [SimplAndUnsafe] *)
-(** changed = false indicates that the topmost implication did not
-change and should be introduced (but potentially more information was
-added after it). *)
-Class SimplImplUnsafe (changed : bool) (P : Prop) (Ps : Prop → Prop) := simpl_impl_unsafe T: (Ps T) → (P → T).
+(** changed = false indicates that P should be introduced into the context in addition to Ps *)
+Class SimplImplUnsafe (changed : bool) (P : Prop) (Ps : Prop) := simpl_impl_unsafe : P → Ps.
 Class SimplAndUnsafe (P : Prop) (Ps : Prop) := simpl_and_unsafe: Ps → P.
 
+Lemma simpl_impl_unsafe_impl changed (P1 P2 T : Prop) `{!SimplImplUnsafe changed P1 P2} :
+  (if changed then (P2 → T) else (P1 → P2 → T)) → (P1 → T).
+Proof. unfold SimplImplUnsafe in *. destruct changed; naive_solver. Qed.
 Lemma simpl_and_unsafe_and (P1 P2 T : Prop) `{!SimplAndUnsafe P1 P2} :
   P2 ∧ T → P1 ∧ T.
 Proof. unfold SimplAndUnsafe in *. naive_solver. Qed.
@@ -27,25 +28,25 @@ Proof. move => ?. by eauto. Qed.
 (** ** [SimplImpl] and [SimplAnd] *)
 (** [SimplImpl] and [SimplAnd] are safe variants which ensure that no
 information is lost. *)
-Class SimplImpl (changed : bool) (P : Prop) (Ps : Prop → Prop) := simpl_impl T: (Ps T) ↔ (P → T).
-Class SimplAnd (P : Prop) (Ps : Prop) := simpl_and: (Ps) ↔ (P).
-Global Instance simplimpl_simplunsafe c P Ps {Hi: SimplImpl c P Ps} :
-  SimplImplUnsafe c P Ps.
+Class SimplImpl (P : Prop) (Ps : Prop) := simpl_impl : Ps ↔ P.
+Class SimplAnd (P : Prop) (Ps : Prop) := simpl_and: Ps ↔ P.
+Global Instance simplimpl_simplunsafe P Ps {Hi: SimplImpl P Ps} :
+  SimplImplUnsafe true P Ps.
 Proof. unfold SimplImpl, SimplImplUnsafe in *. naive_solver. Qed.
 Global Instance simpland_simplunsafe P Ps {Hi: SimplAnd P Ps} :
   SimplAndUnsafe P Ps.
 Proof. unfold SimplAnd, SimplAndUnsafe in *. naive_solver. Qed.
 
 (** ** [SimplImplRel] and [SimplAndRel] *)
-Class SimplImplRel {A} (R : relation A) (changed : bool) (x1 x2 : A) (Ps : Prop → Prop)
-  := simpl_impl_eq T: (Ps T) ↔ (R x1 x2 → T).
+Class SimplImplRel {A} (R : relation A) (changed : bool) (x1 x2 : A) (Ps : Prop)
+  := simpl_impl_eq: Ps ↔ R x1 x2.
 Class SimplAndRel {A} (R : relation A) (x1 x2 : A) (Ps : Prop)
-  := simpl_and_eq: (Ps) ↔ (R x1 x2).
-Global Instance simpl_impl_rel_inst1 {A} c R (x1 x2 : A) Ps `{!SimplImplRel R c x1 x2 Ps} :
-  SimplImpl c (R x1 x2) Ps.
+  := simpl_and_eq: Ps ↔ R x1 x2.
+Global Instance simpl_impl_rel_inst1 {A} R (x1 x2 : A) Ps `{!SimplImplRel R c x1 x2 Ps} :
+  SimplImpl (R x1 x2) Ps.
 Proof. unfold SimplImplRel, SimplImpl in *. naive_solver. Qed.
-Global Instance simpl_impl_rel_inst2 {A} c R (x1 x2 : A) Ps `{!SimplImplRel R c x2 x1 Ps} `{!Symmetric R} :
-  SimplImpl c (R x1 x2) Ps.
+Global Instance simpl_impl_rel_inst2 {A} R (x1 x2 : A) Ps `{!SimplImplRel R c x2 x1 Ps} `{!Symmetric R} :
+  SimplImpl (R x1 x2) Ps.
 Proof. unfold SimplImplRel, SimplImpl in *. naive_solver. Qed.
 Global Instance simpl_and_rel_inst1 {A} R (x1 x2 : A) Ps `{!SimplAndRel R x1 x2 Ps} :
   SimplAnd (R x1 x2) Ps.
@@ -57,10 +58,10 @@ Proof. unfold SimplAndRel, SimplAnd in *. naive_solver. Qed.
 (** ** [SimplBoth] *)
 Class SimplBoth (P1 P2 : Prop) := simpl_both: P1 ↔ P2.
 Global Instance simpl_impl_both_inst P1 P2 {Hboth : SimplBoth P1 P2}:
-  SimplImpl true P1 (λ T, P2 → T).
+  SimplImpl P1 P2.
 Proof. unfold SimplBoth in Hboth. split; naive_solver. Qed.
 Global Instance simpl_and_both_inst P1 P2 {Hboth : SimplBoth P1 P2}:
-  SimplAnd P1 (P2).
+  SimplAnd P1 P2.
 Proof. unfold SimplBoth in Hboth. split; naive_solver. Qed.
 
 (** ** [SimplBothRel] *)
